\documentclass{article}
\usepackage{amsmath}
\usepackage{amssymb}
\usepackage{bm}
\usepackage{verbatim}

\begin{document}

\begin{equation}
f(x) = \frac{1}{2}\left( Ax -b \right)^{T} \left( Ax -b \right) = \frac{1}{2}r^Tr
\end{equation}

\begin{equation}
\nabla f(x) = A^{T}\left( Ax-b\right) = -A^T r
\end{equation}

\begin{eqnarray}
x_{(1)} &=& x_{(0)}  - \alpha \nabla f(x_{(0)}) = \\
&=& x_{(0)} + \alpha A^T r_{(0)}
\end{eqnarray}

\begin{eqnarray}
\frac{d}{d\alpha} f(x_{(1)}) &=& f^{\prime}(x_{(1)})^T \frac{d}{d\alpha} x_{(1)} = \\
&=& f^{\prime}(x_{(1)})^T A^T r_{(0)} = \\
&=& (A^T r_{(1)})^T A^T r_{(0)} = \\
&=&  r_{(1)}^T A A^T r_{(0)} = 0\\
\end{eqnarray}

\begin{eqnarray}
r_{(1)}^T A A^T r_{(0)} &=& 0 \nonumber \\
\left( b - A x_{(1)} \right)^T A A^T r_{(0)} &=& 0 \nonumber \\
\left( b - A \left( x_{(0)} + \alpha A^T r_{(0)} \right) \right)^T A A^T r_{(0)} &=& 0 \nonumber \\
\left( b - A x_{(0)} \right)^T A A^T r_{(0)} - \alpha \left(A A^T r_{(0)}\right)^T A A^T r_{(0)} &=& 0 \nonumber \\
r_{(0)}^T A A^T r_{(0)} &=& \alpha \left(A A^T r_{(0)}\right)^T A A^T r_{(0)} \nonumber  \\
r_{(0)}^T A A^T r_{(0)} &=& \alpha r_{(0)}^T A A^T A A^T r_{(0)} \nonumber \\
\left( A ^T r_{(0)}\right)^T \left(A^T r_{(0)}\right) &=& \alpha \left(A^T r_{(0)}\right)^T A^T A \left(A^T r_{(0)}\right) \nonumber \\
\alpha &=& \frac{\left( A ^T r_{(0)}\right)^T \left(A^T r_{(0)}\right) } {\left(A^T r_{(0)}\right)^T A^T A \left(A^T r_{(0)}\right)} \nonumber
\end{eqnarray}

\end{document}
